Added CPS translation. Utilises coq-ext-lib for monads, etc.

Coq Developments/msci/CPS_Translation.v
@@ -1,12 +1,20 @@
 (** Beginning of the file defining the translation from GV to CP. *)
 Require Import Metatheory.
 Require Import CP_Definitions GV_Definitions.
+Require Import ExtLib.Structures.Applicative.
+Require Import ExtLib.Structures.Functor.
+Require Import ExtLib.Structures.Monad.
+Require Import ExtLib.Data.Option.
+Require Import ExtLib.Data.Monads.OptionMonad.
+Import ApplicativeNotation FunctorNotation MonadNotation.
 Set Implicit Arguments.
+
+Open Scope monad_scope.
 
 (** Translation of types. *)
 Reserved Notation "'⟦' T '⟧t'" (at level 68).
 
-Fixpoint trans_types {k} (T:typ k) : prop :=
+Fixpoint trans_types (T:typ) : prop :=
   match T with
     | ! A # B => (¬ ⟦A⟧t) ⅋ ⟦B⟧t
     | ? A # B => ⟦A⟧t ⨂ ⟦B⟧t
@@ -21,27 +29,135 @@ Fixpoint trans_types {k} (T:typ k) : prop :=
   end
 where "'⟦' T '⟧t'" := (trans_types T).
 
-Program Fixpoint infer (tm:term) (G:tenv) :=
+Fixpoint infer (tm:term) (G:tenv) (xs:list typ) : option typ :=
+  let flip t := match t with
+                   | T ⊸ U => T → U
+                   | T → U => T ⊸ U
+                   | _ => t
+                end
+  in
+  let trans t := match t with
+                     | ! A # B => B
+                     | ? A # B => A <x> A
+                     | _ => t
+                 end
+  in
+  let choose lbl t := match t with
+                        | S1 <+> S2 =>
+                          match lbl with
+                            | lb_inl => S1
+                            | lb_inr => S2
+                          end
+                        | _ => t
+                      end
+  in
   match tm with
     | tm_var (fvar x) => get x G
-    | tm_abs _ T m =>
-    | _ => typ_unit
+    | tm_var (bvar x) => nth_error xs x
+    | tm_unit => Some typ_unit
+    | tm_weak x M => infer M G xs
+    | tm_abs T M => fmap (fun U => T ⊸ U) (infer M G (T::xs))
+    | tm_iabs M => fmap flip (infer M G xs)
+    | tm_eabs M => fmap flip (infer M G xs)
+    | tm_app M N => match infer M G xs with
+                        | Some (T ⊸ U) => Some U
+                        | _ => None
+                    end
+    | tm_pair M N => pure typ_tensor <*> (infer M G xs) <*> (infer N G xs)
+    | tm_let T U M N => infer N G (U::T::xs)
+    | tm_send M N => fmap trans (infer N G xs)
+    | tm_recv M => fmap trans (infer M G xs)
+    | tm_select lbl M => fmap (choose lbl) (infer M G xs)
+    | tm_case M NL NR
+      => T <- fmap (choose lb_inl) (infer M G xs) ;; infer NL G (T::xs)
+    | tm_connect T M N => (infer N G ((dual_session T)::xs))
+    | tm_end _ => Some typ_unit
+  end.
+
+Lemma somm:
+  forall Φ M T (WT: Φ ⊢ M ∈ T), infer M Φ nil = Some T.
+Proof.
+Admitted.
+
+Fixpoint trans_tm' (tm:term) (G:tenv) (xs:list typ) (z:pname) : option proc :=
+  match tm with
+    | tm_var (bvar x)
+    | tm_var (fvar x)
+      => ret $ x ⟷ z
+
+    | tm_unit => ret $ p_accept z pp_top (0 CASE 0)
+
+    | tm_weak (fvar x) M
+    | tm_weak (bvar x) M
+      => M' <- trans_tm' M G xs z ;;
+         ret $ p_weak x M'
+
+    | tm_abs T M
+      => M' <- trans_tm' M G (T::xs) z ;;
+         ret $ p_input z (¬⟦T⟧t) M'
+
+    | tm_iabs M
+      => T  <- infer M G xs ;;
+         M' <- trans_tm' M G xs 0 ;;
+         ret $ p_accept z (⟦T⟧t) M'
+
+    | tm_eabs M
+      => T  <- infer M G xs ;;
+         M' <- trans_tm' M G xs 0 ;;
+         ret $ p_par (pp_accept (⟦T⟧t)) M' (p_request 0 (¬⟦T⟧t) (0 ⟷ z))
+
+    | tm_app M N
+      => TM <- infer M G xs ;;
+         TN <- infer N G xs ;;
+         M' <- trans_tm' M G xs 0 ;;
+         N' <- trans_tm' N G xs 0 ;;
+         ret $ p_par (⟦TM⟧t) M' (p_output 0 (⟦TN⟧t) N' (1 ⟷ z))
+
+    | tm_pair M N
+      => TM <- infer M G xs ;;
+         M' <- trans_tm' M G xs 0 ;;
+         N' <- trans_tm' N G xs z ;;
+         ret $ p_output z (⟦TM⟧t) M' N'
+
+    | tm_let T U M N
+      => M' <- trans_tm' M G xs 0 ;;
+         N' <- trans_tm' N G (U::T::xs) z ;;
+         ret $ p_par (⟦T <x> U⟧t) M' (p_input 0 (¬⟦T⟧t) N')
+
+    | tm_send M N
+      => TM <- infer M G xs ;;
+         TN <- infer N G xs ;;
+         M' <- trans_tm' M G xs 0 ;;
+         N' <- trans_tm' N G xs 0 ;;
+         ret $ p_par (¬⟦TN⟧t) (p_output 0 (⟦TM⟧t) M' (0 ⟷ z)) N'
+
+    | tm_recv M => trans_tm' M G xs z
+
+    | tm_select lbl M
+      => let Q := match lbl with
+                    | lb_inr => p_right
+                    | lb_inl => p_left
+                  end
+         in TM <- infer M G xs ;;
+            M' <- trans_tm' M G xs 0 ;;
+            ret $ p_par (⟦TM⟧t) M' (Q 0 (0 ⟷ z))
+
+    | tm_case M NL NR
+      => TM  <- infer M G xs ;;
+         M'  <- trans_tm' M G xs 0 ;;
+         NL' <- trans_tm' NL G xs z ;;
+         NR' <- trans_tm' NR G xs z ;;
+         ret $ p_par (⟦TM⟧t) M' (p_choice 0 NL' NR')
+
+    | tm_connect T M N
+      => M' <- trans_tm' M G (T::xs) 0 ;;
+         N' <- trans_tm' M G (T::xs) z ;;
+         ret $ p_par (¬⟦T⟧t) (p_par pp_bot M' (p_empout 0)) N'
+
+    | tm_end M
+      => M' <- trans_tm' M G xs 0 ;;
+         ret $ p_par pp_one M' (p_empin 0 (p_accept z pp_top (0 CASE 0)))
   end.
 
 (** Translation of terms. *)
-Reserved Notation "'⟦' t '⟧' z" (at level 68).
-
-Fixpoint trans_tm (tm:term) (z:pname) : proc :=
-  match tm with
-    | tm_var (fvar x) => x ⟷ z
-    | tm_unit => p_accept z pp_top (0 CASE 0)
-    | tm_weak (fvar x) m
-    | tm_weak (bvar x) m =>
-       p_weak x (⟦m⟧ z)
-    | tm_abs _ T m => p_input z (¬⟦T⟧t) (⟦m⟧z)
-    | tm_app m n
-      => p_par (⟦ infer m ⟧t) (⟦m⟧ 0)
-               (p_output 0 (⟦ infer n ⟧t) (⟦n⟧0) (1 ⟷ z))
-    | _ => z ⟷ z
-  end
-where "'⟦' t '⟧' z" := (trans_tm t z).
+Definition trans_tm M G z := trans_tm' M G nil z.
